code/rocq/run_test.v
@@ -50,23 +50,27 @@ Module Test1.
     - apply: expanded_step => //=.
       rewrite /big_or/F/select/=.
       apply: expanded_fail => //=.
-    - rewrite /next_alt//=.
+    - apply: next_alt1 => //=.
     - apply: run_backtrack.
       - apply: expanded_step => //=.
         rewrite /big_or/F/select/= -/s1 -/s2.
         apply: expanded_fail => //=.
-      - rewrite /next_alt//=.
+      - apply: next_alt1 => //=.
       - apply: run_backtrack.
         - apply: expanded_step => //=.
+          apply: expanded_step => //=.
           apply: expanded_fail => //=.
-        - rewrite //=.
+        - apply: next_alt1 => //=.
         - apply: run_backtrack.
           - apply: expanded_step => //=.
+            apply: expanded_step => //=.
             rewrite /big_or/F//=.
             apply: expanded_fail => //=.
-          - move=> //=.
+          - apply: next_alt1 => //=.
           - apply: run_done.
-            by apply: expanded_done.
+            apply: expanded_step => //=.
+            apply: expanded_step => //=.
+            apply: expanded_done => //=.
   Qed.
 End Test1.
 
@@ -99,8 +103,8 @@ Module Test3.
   Lemma xxx {s A A' sA}:
     expand s A = Solved sA A' -> expand sA A' = Failure KO ->
       run s A (Done sA A') ->
-        forall C SC, run s (And A KO C) (Failed SC) -> next_alt s SC = None ->
-          forall D SD, run s (And A KO D) (Failed SD) -> next_alt s SD = None ->
+        forall C SC, run s (And A KO C) (Failed SC) -> next_alt s SC None ->
+          forall D SD, run s (And A KO D) (Failed SD) -> next_alt s SD None ->
             forall B CD0 r s', run s (And (Or A s B) CD0 (Or C sA D)) (Done s' r) ->
               exists r', run s (And B CD0 CD0) (Done s' r').
   Proof.
