code/rocq/valid_state.v
@@ -65,10 +65,12 @@ Module valid_state (U:Unif).
     | Goal _ _ | OK | KO | Bot | Top => true
     | Or l _ r =>
       valid_state l && 
-      if failed l then valid_state r
-      else (base_or r || base_or_ko r)
+      (* if failed l then valid_state r
+      else  *)
+      (base_or r || base_or_ko r)
     | And l r0 r => 
-      valid_state l && if success l || failed l then valid_state r else ((r0 == r) && (base_and r || base_and_ko r))
+      (base_and r0 || base_and_ko r0) &&
+      valid_state l && if success l then valid_state r else ((r0 == r))
     end.
 
   Inductive expandedP (F : state -> bool) : Sigma -> state -> run_res -> Prop :=
@@ -79,8 +81,8 @@ Module valid_state (U:Unif).
 
   Inductive runP (F : state -> bool) : Sigma -> state -> run_res -> Prop :=
     | runP_done {s s' A B}            : F A -> F B -> expandedP F s A (Done s' B) -> runP s A (Done s' B)
-    | runP_fail {s A B}               : F A -> F B -> expandedP F s A (Failed B) -> next_alt s B = None -> runP s A (Failed B)
-    | runP_backtrack {s s' s'' A B C} : F A -> F B -> expandedP F s A (Failed B) -> next_alt s B = Some (s', C) ->  runP s' C s'' -> runP s A s''.
+    | runP_fail {s A B}               : F A -> F B -> expandedP F s A (Failed B) -> next_alt s B None -> runP s A (Failed B)
+    | runP_backtrack {s s' s'' A B C} : F A -> F B -> expandedP F s A (Failed B) -> next_alt s B (Some (s', C)) ->  runP s' C s'' -> runP s A s''.
 
   Lemma full_expanded_cut A: full_expanded (cut A).
   Proof. 
@@ -177,7 +179,8 @@ Module valid_state (U:Unif).
   Proof.
     elim A => //; clear.
     + move=> A HA s B HB; rewrite /base_or => /orP [] //= /andP [] /base_and_valid -> /base_or_aux_base_or.
-      move=> H; move: (H) => /HB ->; rewrite H; case failed => //=.
+      (* move=> H; move: (H) => /HB ->; rewrite H; case failed => //=. *)
+      by move=> /[dup] H => ->.
     + move=> A HA B HB C HC; rewrite /base_or => /orP []//=; case: A HA => //.
       move=> p a H /andP [] /eqP -> H1 ; move:(H1) ->; move: H1 => /base_and_valid ->; rewrite eq_refl.
       case: some_expanded => //.
@@ -187,7 +190,6 @@ Module valid_state (U:Unif).
     expand s A = Solved s' A' -> some_expanded A'.
   Proof.
     elim: A s s' A' => //.
-    + by move=> s s' A [] /[subst2].
     + by move=> s s' A [] /[subst2].
     + by move=> p [].
     + move=> A IHA s B IHB s1 s2 C.
@@ -201,7 +203,6 @@ Module valid_state (U:Unif).
     expand s A = Failure A' -> some_expanded A'.
   Proof.
     elim: A s A' => //.
-    + by move=> s A [] /[subst1].
     + by move=> s A [] /[subst1].
     + by move=> p [].
     + move=> A IHA s B IHB s1 C.
@@ -234,7 +235,7 @@ Module valid_state (U:Unif).
   Qed.
 
 
-  Lemma some_expanded_expanded {s A A'}:
+  (* Lemma some_expanded_expanded {s A A'}:
     expand s A = Expanded A' -> some_expanded A'.
   Proof.
     elim: A s A' => //.
@@ -250,7 +251,7 @@ Module valid_state (U:Unif).
         by rewrite (IHA _ _ HA).
       + move=> [s2 [A' [B' [EA [EB]]]]] /[subst1] /=.
         by rewrite (some_expanded_solved EA).
-  Qed.
+  Qed. *)
 
   Lemma expand_solved_failed {s1 A s2 B}: expand s1 A = Solved s2 B -> failed A = false.
   Proof.
@@ -267,7 +268,18 @@ Module valid_state (U:Unif).
   Proof.
     elim: A s1 s2 B => //.
     + by move=> ??? [] /[subst2].
-    + by move=> ??? [] /[subst2].
+    (* + by move=> ??? [] /[subst2]. *)
+    + by move=> ? [].
+    + move=> A HA s B HB s1 s2 C /= /simpl_expand_or_solved [A' [HA']] /[subst1] /= [].
+      by rewrite (HA _ _ _ HA').
+    + move=> A HA ? _ B HB s1 s2 C /simpl_expand_and_solved [s3 [A' [B' [HA' [HB']]]]] /[subst1] //=.
+      by rewrite (HA _ _ _ HA') (HB _ _ _ HB').
+  Qed.
+
+  Lemma expand_solved_success1 {s1 A s2 B}: expand s1 A = Solved s2 B -> success A.
+  Proof.
+    elim: A s1 s2 B => //.
+    (* + by move=> ??? [] /[subst2]. *)
     + by move=> ? [].
     + move=> A HA s B HB s1 s2 C /= /simpl_expand_or_solved [A' [HA']] /[subst1] /= [].
       by rewrite (HA _ _ _ HA').
@@ -298,8 +310,23 @@ Module valid_state (U:Unif).
       + by move=> [s1 [A' [B' [HA' [+]]]]] ? /= => /HB ->; case success.
   Qed.
 
-  Lemma expand_failure_failed {s1 A B}: expand s1 A = Failure B ->  failed A ->  failed B.
+  Lemma expand_failure_left {s1 A B}:
+    expand s1 A = Failure B -> failed A.
   Proof.
+    elim: A s1 B; clear => //.
+    + by move=> ? [] //.
+    + move=> A HA s1 B HB s2 C /simpl_expand_or_fail [A' [HA']] /[subst1].
+      apply: HA HA'.
+    + move=> A HA B0 _ B HB s C /simpl_expand_and_fail [].
+      + move=> [A'[HA']]  /[subst1] /=.
+        by rewrite (HA _ _ HA').
+      + move=> [s' [A' [B' [HA' [HB']]]]] /[subst1] /=.
+        by rewrite (HB _ _ HB') (expand_solved_success1 HA') orbT.
+  Qed.
+
+  Lemma expand_failure_failed {s1 A B}: expand s1 A = Failure B -> failed B.
+  Proof.
+    move=> /[dup] + /expand_failure_left.
     elim: A s1 B => //.
     + by move=> ?? [] /[subst2].
     + move=> A HA s B HB s1 C /= /simpl_expand_or_fail [A' [HA']] /[subst1] /=.
@@ -315,47 +342,48 @@ Module valid_state (U:Unif).
           by rewrite (expand_solved_success HA') (HB _ _ HB' FB) orbT.
   Qed.
 
+  Lemma base_and_ko_valid {B}: base_and_ko B -> valid_state B.
+  Proof. 
+    elim: B => // A HA B HB C HC /=.
+    destruct A => // /andP [] /eqP -> /[dup] /HC -> ->.
+    by rewrite eq_refl orbT.
+  Qed.
+
+  Lemma base_and_base_and_ko_valid {B}:
+    base_and B || base_and_ko B -> valid_state B.
+  Proof. by move=> /orP []; [move=> /base_and_valid | move=> /base_and_ko_valid] => ->. Qed.
+
   Lemma base_or_ko_valid {B}: base_or_ko B -> valid_state B.
   Proof.
     rewrite /base_or_ko => /orP [].
     + by move=> /eqP ->.
     + elim: B => //.
-      + move=> [] => //.
-        move=> [] => // B C // /= + _ D H /andP [] /andP [] /eqP H1 H2.
-        by rewrite H1 eq_refl H2 => /(_ isT) -> /H ->.
-      + by move=> [] // HA B0 HB0 B H /= /andP [] _; case: B H => //.
+      + move=> A HA s B HB /= /andP [] /base_and_ko_valid ->.
+        rewrite /base_or_ko /base_or.
+        case: B {HB} => //=.
+        + by move=> C _ D ->; rewrite orbT.
+        + move=> [] //.
+      + by move=> [] // HA B0 HB0 B HB /= /andP [] /[dup] /eqP -> -> ->; rewrite orbT.
   Qed.
 
   Lemma base_or_base_or_ko_valid {B}:
     base_or B || base_or_ko B -> valid_state B.
   Proof. by move=> /orP []; [move=> /base_or_valid | move=> /base_or_ko_valid] => ->. Qed.
 
-  Lemma base_and_ko_valid {B}: base_and_ko B -> valid_state B.
-  Proof. by elim: B=> // -[] //= _ B HB C HC /andP [] _ /HC. Qed.
-
-  Lemma base_and_base_and_ko_valid {B}:
-    base_and B || base_and_ko B -> valid_state B.
-  Proof. by move=> /orP []; [move=> /base_and_valid | move=> /base_and_ko_valid] => ->. Qed.
-
   Lemma valid_state_solved {s s' A A'}:
     expand s A = Solved s' A' -> valid_state A -> valid_state A'.
   Proof.
     elim: A s s' A' => //.
     + by move=> s s' A [] /[subst2].
-    + move=> s s' A //= [] /[subst2] //=. 
     + by move=> pr [] => //= t s s' A'; case: F => //= -[].
     + move=> A IHA s B IHB s1 s2 C.
-      move=> /simpl_expand_or_solved [A' []] /[dup] H /IHA HP /[subst1] /= /andP [] /[dup] VA => {}/HP ->.
-      rewrite (expand_solved_failed H) => /[dup] /base_or_base_or_ko_valid -> ->.
-      by case: failed.
+      by move=> /simpl_expand_or_solved [A' []] /[dup] H /IHA HP /[subst1] /= /andP [] /[dup] VA => {}/HP -> ->.
     + move=> A IHA B0 _ B IHB s1 s2 C /simpl_expand_and_solved [s' [A'[B'[HA[HB]]]]] /[subst1] /=.
       rewrite (expand_solved_success HA).
-      move=> /andP [] VA; rewrite (IHA _ _ _ HA VA).
+      move=> /andP [] /andP [] /[dup] BB0 -> /[dup] /(IHA _ _ _ HA) -> VA.
       case SA: success.
       + by move=> VB; rewrite (IHB _ _ _ HB VB).
-      + move=> /=; case X: failed.
-        + by move=> /(IHB _ _ _ HB).
-        + by move=> /andP [] _ /base_and_base_and_ko_valid /(IHB _ _ _ HB).
+      + by move=> /eqP H; rewrite H in BB0; move: BB0 => /base_and_base_and_ko_valid /(IHB _ _ _ HB) ->.
   Qed.
 
   Lemma valid_state_failure {s A A'}:
@@ -363,30 +391,22 @@ Module valid_state (U:Unif).
   Proof.
     elim: A s A' => //.
     + by move=> s A [] /[subst2].
-    + move=> s A //= [] /[subst2] //=. 
     + by move=> pr [] => //= t s A'; case: F => //= -[].
     + move=> A IHA s B IHB s1 C.
       move=> /simpl_expand_or_fail [A' [HA]] /[subst1] //= /andP [] VA.
-      rewrite (IHA _ _ HA VA).
-      case X: failed => /[dup] H ->.
-      + by rewrite (expand_failure_failed HA X).
-      + by move: H => /orP []; [move=> /base_or_valid | move=> /base_or_ko_valid] => ->; case failed.
+      by rewrite (IHA _ _ HA VA) => ->.
     + move=> A IHA B0 _ B IHB s1 C /simpl_expand_and_fail [].
-      + move=> [A' [HA]] /[subst1] //= /andP [] VA.
+      + move=> [A' [HA]] /[subst1] //= /andP [] /andP [] HB0 VA.
         rewrite (expand_failure_success HA)/=.
-        rewrite (IHA _ _ HA VA).
-        case X: failed.
-        + by rewrite (expand_failure_failed HA X) orbT => ->.
-        + move=> /andP [] -> /[dup] /base_and_base_and_ko_valid -> ->.
-          by case: success => //=; case failed.
-      + move=> [s' [A' [B' [HA [HB]]]]] /[subst1] /= /andP [] VA.
+        move=> /eqP /[subst1].
+        rewrite (IHA _ _ HA VA) HB0 eq_refl (base_and_base_and_ko_valid HB0).
+        by case: success => //=.
+      + move=> [s' [A' [B' [HA [HB]]]]] /[subst1] /= /andP [] /andP [] HB0 VA.
         rewrite (expand_solved_success HA).
         rewrite (valid_state_solved HA VA) => {HA VA}.
         case X: success => /=.
-        + by move=> /(IHB _ _ HB) ->.
-        + case Y: failed.
-          + by move=> /(IHB _ _ HB).
-          + by move=> /andP [] _ /base_and_base_and_ko_valid /(IHB _ _ HB).
+        + by move=> /(IHB _ _ HB) ->; rewrite HB0.
+        + by move=> /eqP /[subst1]; rewrite HB0 (IHB _ _ HB (base_and_base_and_ko_valid HB0)).
   Qed.
 
   Lemma expand_cb_failed {s1 A A'}: expand s1 A = CutBrothers A' -> failed A = false.
@@ -407,14 +427,13 @@ Module valid_state (U:Unif).
     + move=> A IHA s B IHB s1 C.
       by move=> /simpl_expand_or_cut.
     + move=> A IHA B0 _ B IHB s1 C /simpl_expand_and_cut [].
-      + move=> [A' [HA]] /[subst1] //= /andP [] /(IHA _ _ HA) ->.
-        rewrite (expand_cb_success HA) (expand_cb_failed HA) => /= /andP [] -> /[dup] /base_and_base_and_ko_valid -> ->.
-        by case: orb.
-      + move=> [s' [A' [B' [HA [HB]]]]] /[subst1] /= /andP [] /(valid_state_solved HA) ->.
-        rewrite (expand_solved_success HA) (expand_solved_failed HA).
+      + move=> [A' [HA]] /[subst1] //= /andP [] /andP [] HB0 /(IHA _ _ HA) ->.
+        by rewrite (expand_cb_success HA) => /eqP /[subst1]; rewrite HB0 eq_refl (base_and_base_and_ko_valid HB0); case: success.
+      + move=> [s' [A' [B' [HA [HB]]]]] /[subst1] /= /andP [] /andP [] HB0 /(valid_state_solved HA) ->.
+        rewrite (expand_solved_success HA).
         case X: success => /=.
-        + by move=> /(IHB _ _ HB) ->.
-        + by move=> /andP [] _ /base_and_base_and_ko_valid /(IHB _ _ HB).
+        + by move=> /(IHB _ _ HB) ->; rewrite HB0.
+        + by move=> /eqP /[subst1]; rewrite (IHB _ _ HB (base_and_base_and_ko_valid HB0)) HB0.
   Qed.
 
   Lemma full_expanded_big_and {pr l}:
@@ -426,16 +445,15 @@ Module valid_state (U:Unif).
     elim: l s => [|[]] //=.
     + move=> s; rewrite valid_state_big_and // full_expanded_big_and.
     + move=> _ r l IH s.
-      rewrite base_or_big_or_aux valid_state_big_and IH.
-      by case failed.
+      by rewrite valid_state_big_and base_or_big_or_aux.
   Qed.
 
   Lemma valid_state_big_or {pr s t} : valid_state (big_or pr s t).
   Proof.
     case: t; rewrite /big_or//=.
-    + by move=> ?; case: F => //= -[] //=???; rewrite valid_state_big_or_aux.
-    + by move=> ?; case: F => //= -[] //=???; rewrite valid_state_big_or_aux.
-    + by move=> ??; case F => //= -[] //=???; rewrite valid_state_big_or_aux.
+    + by move=> ?; case: F => //= -[] //=???; rewrite base_or_big_or_aux.
+    + by move=> ?; case: F => //= -[] //=???; rewrite base_or_big_or_aux.
+    + by move=> ??; case F => //= -[] //=???; rewrite base_or_big_or_aux.
   Qed. 
 
   Lemma full_expanded_cb {s1 A A'} : 
@@ -508,20 +526,6 @@ Module valid_state (U:Unif).
   Lemma simpl_and_cut {A B C}: cut (And A B C) = And (cut A) (cut B) (cut C).
   Proof. by []. Qed.
 
-  Lemma valid_state_valid_state_cut {B}: valid_state B -> valid_state (cut B).
-  Proof.
-    elim: B => //.
-    + move=> A IHA s B IHB /= /andP [] /IHA ->.
-      rewrite failed_cut; case: failed.
-      + by move=> /IHB ->.
-      + by move=> /base_or_base_or_ko_valid /IHB ->.
-    + move=> A HA B HB C HC => /= /andP [] /HA /= ->.
-      rewrite success_cut failed_cut/=.
-      case X: orb.
-      + by move=> /HC.
-      + by move=> /andP [] _ /base_and_base_and_ko_valid /HC.
-  Qed.
-
   Lemma base_and_ko_cut {B}: base_and_ko B -> base_and_ko (cut B).
   Proof.
     elim: B => //.
@@ -548,26 +552,25 @@ Module valid_state (U:Unif).
   Proof.
     elim: A s A' => //.
     + by move=> pr [] => //= t s ? [] /[subst1]; rewrite valid_state_big_or.
+    + by move=> s A [] <-.
+    + by move=> s [] ?? // ? [] <-; rewrite valid_state_big_or.
     + move=> A IHA s B IHB s1 C.
       move=> /simpl_expand_or_expanded [].
       + move=> [A' [/[dup] H]] + /[subst1] /= => + /andP [] /(IHA _ _ H) ->.
-        move=> /expand_expanded_failed -> /[dup] /base_or_base_or_ko_valid -> ->.
-        by case failed.
+        by move=> _ ->.
       + move=> [A' [HA']] /[subst1] /= /andP [] /(valid_state_cb HA') ->.
-        rewrite (expand_cb_failed HA') => /[dup] /base_or_base_or_ko_valid /valid_state_valid_state_cut -> H.
+        move=> H.
         have: base_or (cut B) || base_or_ko (cut B).
           by move: H => /orP []; [move=> /base_or_base_or_ko_cut | move=>/base_or_ko_cut] => ->; rewrite orbT.
-        by move=> ->; case failed.
+        by move->.
     +  move=> A IHA B0 _ B IHB s1 C /simpl_expand_and_expanded [].
-      + move=> [A' [HA]] /[subst1] //= /andP [] /(IHA _ _ HA) ->.
-        rewrite (expand_expanded_success HA) (expand_expanded_failed HA) /=.
-        move => /andP [] /eqP <- /[dup] /base_and_base_and_ko_valid -> ->.
-        by rewrite eq_refl; case orb.
-      + move=> [s' [A' [B' [HA [HB]]]]] /[subst1] /= /andP [] /(valid_state_solved HA) ->.
+      + move=> [A' [HA]] /[subst1] //= /andP [] /andP [] /[dup] /base_and_base_and_ko_valid VB0 -> /(IHA _ _ HA) ->.
+        by rewrite (expand_expanded_success HA) /= => /eqP /[subst1]; rewrite eq_refl VB0; case success.
+      + move=> [s' [A' [B' [HA [HB]]]]] /[subst1] /= /andP [] /andP [] /[dup] /base_and_base_and_ko_valid VB -> /(valid_state_solved HA) ->.
         rewrite (expand_solved_success HA) /=.
-        case X: orb.
+        case X: success.
         + by move=> /(IHB _ _ HB) ->.
-        + by move=> /andP [] _ /base_and_base_and_ko_valid /(IHB _ _ HB) H; rewrite H.
+        + by move=> /eqP /[subst1]; rewrite (IHB _ _ HB VB).
   Qed.
 
   Lemma expandedP_expanded {s A r}:
@@ -601,7 +604,7 @@ Module valid_state (U:Unif).
       by move=> /(_ _ _ erefl VB).
   Qed.
 
-  Lemma valid_state_expanded_failed {s1 A B}:
+  Lemma valid_state_expanded_valid_state {s1 A B}:
     valid_state A ->  expanded s1 A (Failed B) -> valid_state B.
   Proof.
     remember (Failed _) as D eqn:HD => + H.
@@ -614,69 +617,84 @@ Module valid_state (U:Unif).
       by move=> /(_ _ erefl VB).
   Qed.
 
-  Lemma next_alt_cut {b s B}: next_alt_aux b s (cut B) = None.
+  Lemma valid_state_expanded_failed {s A B}:
+    valid_state A -> expanded s A (Failed B) -> failed B.
   Proof.
-    elim: B s b => //; clear.
-    + by move=> A HA s B HB s1 b /=; rewrite HA failed_cut HB.
-    + by move=> A HA B HB C HC s b /=; rewrite HC HA.
+    remember (Failed _) as F eqn:HF => + H.
+    elim: H B HF; clear => //.
+    + move=> s A B H ? [] <-.
+      elim: A s B H; clear => //.
+      + by move=> s B [] /[subst1].
+      + by move=> p [] s B //=.
+      + move=> A HA s B HB s1 C /simpl_expand_or_fail [A' [H]] /[subst1].
+        move=> /=/andP[] /(HA _ _ H) FA.
+        by rewrite (expand_failure_failed H).
+      + move=> A HA B0 _ B HB s C /simpl_expand_and_fail [].
+        + by move=> [A'[HA']] /[subst1] /=/andP [] /andP [] /[dup] /base_and_base_and_ko_valid VB0 H; rewrite (expand_failure_success HA') => /(HA _ _ HA') -> /=.
+        + by move=> [s'[A'[B'[HA'[HB']]]]] /[subst1] /=; rewrite (expand_failure_failed HB') (expand_solved_success HA') orbT.
+    + move=> ???? H H1 IH ? /[subst1] H2; apply: IH erefl (valid_state_cb H H2).
+    + move=> ???? H H1 IH ? /[subst1] H2; apply: IH erefl (valid_state_expanded H H2).
   Qed.
 
-  (* Lemma next_alt_aux_not_cut {b s1 C}: (C == cut C) = false -> exists s2 B, next_alt_aux b s1 C = Some (s2, B).
+  Lemma next_alt_aux_base_and {s1 s2 A B}:
+     base_and A || base_and_ko A ->  next_alt_aux true s1 A = Some (s2, B) -> A = B.
   Proof.
-    elim: C b s1 => //=.
-    + move=> _ _ _*)
+    elim: A s1 s2 B => //; move=> [] //.
+    + move=> _ B0 HB0 B HB s1 s2 C /= /andP [] /eqP /[subst1] BA.
+      case NB: next_alt_aux => // [[ ]] [] /[subst2].
+      rewrite BA in HB.
+      by rewrite (HB _ _ _ (orbT _) NB).
+    + move=> p a _ B0 HB0 B HB s1 s2 C /= /orP []// /andP []/eqP/[subst1] BB.
+      case NB: next_alt_aux => // [[ ]] [] /[subst2].
+      by rewrite BB in HB; rewrite (HB _ _ _ isT NB).
+  Qed.
 
-  Lemma next_alt_failed1 {b s1 s2 A B}: valid_state A -> next_alt_aux b s1 A = Some (s2, B) -> failed B = false.
-  Proof.
-    elim: A b s1 s2 B => //=.
-    + by  move=>b; case: b => //= ??? _ [] /[subst2].
-    + move=>b; case: b => //= ??? _ [] /[subst2] //=.
-    + move=>p a b; case: b => //= ??? _ [] /[subst2] //.
-    + move=> A HA s B HB _ s1 s2 C; case NA: next_alt_aux => [[ ]|].
-      + by move=> /andP [] VA _ [] /[subst2] /=; rewrite (HA _ _ _ _ _ NA).
-      + move=> /andP [] VA FVA.
-        have {FVA} VB: valid_state B.
-          move: FVA; case: failed => //; apply: base_or_base_or_ko_valid.
-        case FB: failed.
-        + by move=> /(HB _ _ _ _ VB).
-        + by move=> [] /[subst2].
-    + move=> A HA B0 HB0 B HB /= _ s1 s2 D.
-      move=> /andP [] VA SFA.
-      have {SFA} VB : valid_state B.
-        move: SFA; case: orb => // /andP [] _; apply base_and_base_and_ko_valid.
-      case NB: next_alt_aux => /= [[ ]|].
-      + move=> []/[subst2] /=.
-        rewrite (HB _ _ _ _ VB NB).
-        admit.
-      + case NA: next_alt_aux => /= [[ ]|] => //.
-        move=> [] /[subst2] /=.
-  Admitted.
-
-  Lemma next_alt_failed {b s1 s2 A B}: valid_state A -> next_alt_aux b s1 A = Some (s2, B) -> failed A = false.
+  Lemma next_alt_failed {b s1 s2 A B}: 
+    valid_state A -> next_alt_aux b s1 A = Some (s2, B) 
+    -> valid_state B.
   Proof.
     elim: A b s1 s2 B => //.
-    + admit.
-    + move=> A HA B HB C HC /= _ s1 s2 D /andP [] VA.
-      case SF: orb.
-  Admitted.
+    + by move=> [] // ??? _ [] /[subst2].
+    + by move=> [] // ??? _ [] /[subst2].
+    + by move=> ?? [] // ??? _ [] /[subst2].
+    + move=> A HA s B HB b s1 s2 C /= /andP [] VA /[dup] /base_or_base_or_ko_valid VB BO.
+      case NA: next_alt_aux => [[s3 A']|] [] /[subst2] //=.
+      by rewrite (HA _ _ _ _ VA NA) BO.
+    + move=> A HA B0 HB0 B HB b s1 s2 C.
+      move=> /= /andP [] /andP [] /[dup] /base_and_base_and_ko_valid VB0 H VA.
+      case SA: success.
+      (* case AND A B *)
+      + (* case success or failed A *)
+        move=> VB.
+        case NB: next_alt_aux => [[ ]|].
+        + by move=> [] /[subst2] /= ; rewrite VA (HB _ _ _ _ VB NB) SA H.
+        + case NA: next_alt_aux => [[ ]|] // [] /[subst2] /=.
+           by rewrite (HA _ _ _ _ VA NA) eq_refl H VB0; case success.
+      + move=> /eqP /[subst1].
+        case NB: next_alt_aux => [[s3 D]|].
+        + move=> [] /[subst2] /=; rewrite VA (HB _ _ _ _ (base_and_base_and_ko_valid H) NB) SA.
+          rewrite H.
+          by rewrite (next_alt_aux_base_and H NB) eq_refl.
+        + case NA: next_alt_aux => // [[ ]] [] /[subst2] /=.
+          by rewrite (HA _ _ _ _ VA NA) eq_refl (base_and_base_and_ko_valid H) H; case success.
+  Qed.
 
-  Lemma valid_state_next_alt {s s' b A B} : next_alt_aux b s A = Some (s', B) -> valid_state A -> valid_state B.
+  Lemma valid_state_next_alt {s s' A B} : 
+    failed A ->
+    next_alt s A (Some (s', B)) -> valid_state A ->  valid_state B.
   Proof.
-    elim: A b s s' B => //.
-    + by move=> [] ??? // [] /[subst2].
-    + by move=> [] ??? // [] /[subst2].
-    + by move=> ? [|?] [] // ??? -[] /[subst2].
-    + move=> A HA s B HB b s1 s2 C /= + /andP [] VA.
-      case FA: failed => + VB.
-      case F: next_alt_aux => [[ ]| ].
-      + move=> [] /[subst2].
-
-        admit.
-      (* + case X: eq_op => // -[] /[subst2]. *)
-        admit.
-    + admit.
-  Admitted.
-
+    remember (Some _) as S eqn:HS.
+    move=> + H; elim: H s' B HS => //; clear.
+    + move=> s s2 A B' + FB s1 B [] /[subst2].
+      by move=> /next_alt_failed H1.
+       (* /H1 {}H1 /H1. *)
+    + move=> s s1 s2 A B C + FB HB s3 D [] /[subst2].
+      move=> /next_alt_failed H1.
+      move=> ?.
+      move=> /H1.
+       (* /H1 {}H1 /H1 /next_alt_failed H. *)
+      by move: HB => /next_alt_failed H /H.
+  Qed.
 
   Lemma runP_run {s A r}:
     valid_state A -> run s A r -> runP valid_state s A r.
@@ -688,12 +706,14 @@ Module valid_state (U:Unif).
       apply: runP_done => //.
     + move=> s A B HA HB VA.
       have:= expandedP_expanded VA HA => H.
-      have VS := valid_state_expanded_failed VA HA.
+      have VS := valid_state_expanded_valid_state VA HA.
       apply: runP_fail => //.
     + move=> s s' r A B C HA HB HC IH VA.
       have EA := expandedP_expanded VA HA.
-      have VB := valid_state_expanded_failed VA HA.
-      have NA := valid_state_next_alt HB VB.
+      have VB := valid_state_expanded_valid_state VA HA.
+      have FB := valid_state_expanded_failed VA HA.
+      have NA := valid_state_next_alt FB HB VB.
+      (* have NNA := base_or_base_or_ko_valid NA. *)
       apply: runP_backtrack VA VB EA HB (IH NA).
   Qed.
 
